scripts/check-mrdt-refactor.sh
@@ -1,0 +1,4 @@
+#!/usr/bin/env sh
+set -eu
+
+lake build Sal.MRDTs.Metatheory.RefactorLedger
